proving the functional correctness of median(s)

examples/wysteria/examples/mediantuple.fst
@@ -3,10 +3,11 @@
     other-files:ghost.fst ext.fst set.fsi heap.fst st.fst all.fst io.fsti list.fst st2.fst ordset.fsi ../prins.fsi ffi.fst wysteria.fsi
  --*)
 
-(* Millionaire's with 2 parties *)
+(* Median *)
 
 module SMC
 
+open Prins
 open FFI
 open Wysteria
 
@@ -17,40 +18,109 @@ let ab = union alice_s bob_s
 type pre  (m:mode)  = fun m0 -> b2t (m0 = m)
 type post (#a:Type) = fun (m:mode) (x:a) (t:trace) -> True
 
-val read_fn: unit -> Wys (int * int) (fun m0 -> Mode.m m0 = Par /\
-                                        (exists p. Mode.ps m0 = singleton p))
-                                (fun m0 r t -> True)
-let read_fn x = w_read_int_tuple ()
+val read_fn: unit -> Wys int (fun m0 -> Mode.m m0 = Par /\
+                                 (exists p. Mode.ps m0 = singleton p))
+                          (fun m0 r t -> True)
+let read_fn x = w_read_int ()
 
-val median: unit -> Wys int (pre (Mode Par ab)) post
-let median _ =
-  let p_alice = as_par alice_s read_fn in
-  let p_bob = as_par bob_s read_fn in
+type distinct (x1:int) (x2:int) (y1:int) (y2:int) =
+  x1 =!= x2 /\ x1 =!= y1 /\ x1 =!= y2 /\ x2 =!= y1 /\ x2 =!= y2 /\ y1 =!= y2
 
-  let tup = mk_tuple p_alice p_bob in
+type eq_one (n:int) (x1:int) (x2:int) (x3:int) (x4:int) = n = x1 \/ n = x2 \/ n = x3 \/ n = x4
+
+assume val sort: x1:int -> x2:int -> y1:int -> y2:int{distinct x1 x2 y1 y2}
+                 -> GTot (r:(int * int * int * int){MkTuple4._1 r < MkTuple4._2 r      /\
+		                           MkTuple4._2 r < MkTuple4._3 r      /\
+					   MkTuple4._3 r < MkTuple4._4 r      /\
+					   eq_one (MkTuple4._1 r) x1 x2 y1 y2 /\
+					   eq_one (MkTuple4._2 r) x1 x2 y1 y2 /\
+					   eq_one (MkTuple4._3 r) x1 x2 y1 y2 /\
+					   eq_one (MkTuple4._4 r) x1 x2 y1 y2})
+
+val median_spec: x1:int -> x2:int -> y1:int -> y2:int{distinct x1 x2 y1 y2} -> GTot int
+let median_spec x1 x2 y1 y2 =
+  let p = sort x1 x2 y1 y2 in
+  MkTuple4._2 p
+
+val monolithic_median: x1:int -> x2:int -> y1:int -> y2:int -> Tot int
+let monolithic_median x1 x2 y1 y2 =
+  let a = x1 <= y1 in
+  let x3 = if a then x2 else x1 in
+  let y3 = if a then y1 else y2 in
+  let d = x3 <= y3 in
+  if d then x3 else y3
+
+type median_pre (x1:int) (x2:int) (y1:int) (y2:int) =
+  x1 < x2 /\ y1 < y2 /\ distinct x1 x2 y1 y2
+
+val monolithic_median_correctness:
+  x1:int -> x2:int -> y1:int -> y2:int
+  -> Lemma (requires (True))
+          (ensures (median_pre x1 x2 y1 y2 ==> monolithic_median x1 x2 y1 y2 =
+	                                      median_spec x1 x2 y1 y2))
+let monolithic_median_correctness x1 x2 y1 y2 = ()
+
+val mono_median: unit -> Wys int (pre (Mode Par ab)) post
+let mono_median _ =
+  let x1 = as_par alice_s read_fn in
+  let x2 = as_par alice_s read_fn in
+  let y1 = as_par bob_s read_fn in
+  let y2 = as_par bob_s read_fn in
 
   let g:unit -> Wys int (pre (Mode Sec ab)) post =
-    fun _ ->
-      let p_alice = fst tup in
-      let p_bob = snd tup in
-      let a_t = unbox_s p_alice in
-      let b_t = unbox_s p_bob in
-      let x1 = fst a_t in
-      let x2 = snd a_t in
-      let y1 = fst b_t in
-      let y2 = snd b_t in
-      let t1 = mk_tuple x1 y1 in
-      let x1 = fst t1 in
-      let y1 = snd t1 in
-      let b1 = x1 <= y1 in
-      let x3 = if b1 then x2 else x1 in
-      let y3 = if b1 then y1 else y2 in
-      let b2 = x3 <= y3 in
-      if b2 then x3 else y3
+    fun _ -> monolithic_median (unbox_s x1) (unbox_s x2) (unbox_s y1) (unbox_s y2)
+  in
+  
+  as_sec ab g
+
+val opt_median: unit -> Wys int (pre (Mode Par ab)) post
+let opt_median _ =
+  let x1 = as_par alice_s read_fn in
+  let x2 = as_par alice_s read_fn in
+  let y1 = as_par bob_s read_fn in
+  let y2 = as_par bob_s read_fn in
+
+  let cmp:
+    x:Box int alice_s -> y:Box int bob_s -> unit
+    -> Wys bool (pre (Mode Sec ab)) (fun _ r _ ->
+    	                            b2t (r = ((v_of_box x) <= (v_of_box y)))) =
+    fun x y _ -> (unbox_s x) <= (unbox_s y)
   in
 
-  as_sec ab g
+  let select:
+    #p:prin -> b:bool -> n1:Box int (singleton p) -> n2:Box int (singleton p) -> unit
+    -> Wys int (pre (Mode Par (singleton p)))
+            (fun _ r _ -> (b       ==> r = v_of_box n1) /\
+	               ((not b) ==> r = v_of_box n2)) =
+    fun #p b n1 n2 _ -> if b then (unbox_p n1) else (unbox_p n2)
+  in
+
+  let select_s:
+    b:bool -> n1:Box int alice_s -> n2:Box int bob_s -> unit
+    -> Wys int (pre (Mode Sec ab))
+            (fun _ r _ -> (b       ==> r = v_of_box n1) /\
+	               ((not b) ==> r = v_of_box n2)) =
+    fun b n1 n2 _ -> if b then (unbox_s n1) else (unbox_s n2)
+  in
+
+  let g:
+    unit -> Wys int (pre (Mode Par ab))
+                 (fun _ r _ -> b2t (r = monolithic_median (v_of_box x1) (v_of_box x2)
+		                                       (v_of_box y1) (v_of_box y2))) =
+    fun _ ->
+      let a = as_sec ab (cmp x1 y1) in
+      let x3 = as_par alice_s (select #alice a x2 x1) in
+      let y3 = as_par bob_s (select #bob a y1 y2) in
+      let d = as_sec ab (cmp x3 y3) in
+      let r = as_sec ab (select_s d x3 y3) in
+      r
+
+  in
+
+  unbox_p (as_par ab g)
 ;;
 
-let x = main ab median in
-print_int x
+let x = main ab mono_median in
+print_int x;
+let y = main ab opt_median in
+print_int y
